Proved general form of bitcoin mulmod algorithm.  Added appropriate hypotheses.

src/BitcoinMultiplication/GeneralizedMultiplicationAlgorithm.v
@@ -2,6 +2,7 @@ Require Import Crypto.Arithmetic.Core.
 Require Import Coq.ZArith.ZArith Coq.micromega.Lia.
 Require Import Coq.Structures.Orders.
 Require Import Coq.Lists.List.
+Require Import Coq.Numbers.NatInt.NZPow.
 Require Import Crypto.Algebra.Nsatz.
 Require Import Crypto.Arithmetic.ModularArithmeticTheorems.
 Require Import Crypto.Util.Decidable.
@@ -49,6 +50,78 @@ Import Compilers.API.
 Import Associational Positional HelpfulFunctions.
 Import ListNotations. Local Open Scope Z_scope.
 
+Notation "a ** b" := (Zpower_nat a b)
+  (at level 41, right associativity).
+
+Context 
+        (e : nat)
+        (c : Z)
+        (p_nz : 2 ** e - c <> 0)
+        (limbs : nat)
+        (limb_size : nat)
+        (limbs_gteq_3 : (limbs >= 3)%nat)
+        (e_small : (e <= limb_size * limbs)%nat)
+        (e_big : (limb_size * (limbs - 1) <= e)%nat).
+
+Definition s := 2 ** e.
+
+Definition base := 2 ** limb_size.
+
+Lemma base_nz : base <> 0.
+Proof. cbv [base]. rewrite Zpower_nat_Z. apply Z.pow_nonzero; lia. Qed.
+
+Lemma s_nz : s <> 0.
+Proof. cbv [s]. rewrite Zpower_nat_Z. apply Z.pow_nonzero; lia. Qed.
+
+Definition weight n : Z := base ** n.
+
+Lemma weight_0 : weight 0 = 1.
+Proof. reflexivity. Qed.
+
+Lemma weight_nz : forall i, weight i <> 0.
+Proof.
+  intros i. cbv [weight]. rewrite Zpower_nat_Z. apply Z.pow_nonzero.
+  - apply base_nz.
+  - lia.
+Qed.
+
+Lemma mod_is_zero : forall b (n m : nat), b <> 0 -> le n m -> (b ** m) mod (b ** n) = 0.
+  intros b n m H1 H2. induction H2.
+  - rewrite Z_mod_same_full. constructor.
+  - rewrite Zpower_nat_succ_r. rewrite Z.mul_mod_full. rewrite IHle. rewrite Z.mul_0_r.
+    apply Z.mod_0_l. rewrite Zpower_nat_Z. apply Z.pow_nonzero; lia.
+Qed.
+
+Check Z_div_le.
+
+Lemma div_nz a b : b > 0 -> b <= a -> a / b <> 0.
+Proof.
+  intros H1 H2. assert (1 <= a / b).
+  - replace 1 with (b / b).
+    + apply Z_div_le.
+      -- apply H1.
+      -- apply H2.
+    + apply Z_div_same. apply H1.
+  - symmetry. apply Z.lt_neq. Search ((_ <= _) -> (_ < _)). apply Z.lt_le_trans with 1.
+    + reflexivity.
+    + apply H.
+Qed.
+
+Lemma pow_mul a b c : (a ** b) ** c = a ** (b * c).
+Proof.
+  repeat rewrite Zpower_nat_Z. rewrite Nat2Z.inj_mul. rewrite Z.pow_mul_r.
+  - reflexivity.
+  - apply Zle_0_nat.
+  - apply Zle_0_nat.
+Qed.
+
+Lemma limbs_mod_s_0 : (weight limbs) mod s = 0.
+Proof.
+  cbv [weight base s]. rewrite pow_mul. apply mod_is_zero.
+  - lia.
+  - apply e_small.
+Qed.
+
 Local Open Scope nat_scope.
 
 (* want to start with i = 1 (up to l - 2, excludsive), so want to start with l_minus_2_minus_i = l - 2 - 1 *)
@@ -66,21 +139,49 @@ Fixpoint loop l weight s c l_minus_2_minus_i r0 :=
 Definition reduce' x1 x2 x3 x4 x5 := collect_terms (reduce_one x1 x2 x3 x4 x5).
 Definition carry' x1 x2 x3 := collect_terms (Associational.carry x1 x2 x3).
 
-Definition loop_body limbs weight s c i before :=
+Definition loop_body i before :=
   let middle1 := carry' (weight (i + limbs)) (weight 1) before in
   let middle2 := reduce' s (weight (i + limbs)) (weight limbs) c middle1 in
   let after := carry' (weight i) (weight 1) middle2 in
   after.
+
+Lemma eval_mod_loop_body i before :
+  (Associational.eval (loop_body i before) mod (s - c) =
+  Associational.eval before mod (s - c))%Z.
+Proof.
+  cbv [loop_body carry' reduce'].
+  repeat (try rewrite eval_reduce_one;
+          try rewrite Associational.eval_carry;
+          try rewrite eval_collect_terms).
+  reflexivity.
+  - apply weight_nz.
+  - apply s_nz.
+  - apply weight_nz.
+  - cbv [weight]. apply mod_is_zero.
+    + apply base_nz.
+    + lia.
+  - cbv [weight]. apply limbs_mod_s_0.
+  - apply p_nz.
+  - apply weight_nz.
+Qed.
 
 Definition from_n_to_one n :=
   fold_right (fun (x :nat) l' => (length l' + 1) :: l') [] (repeat 0 n).
 
 Compute (from_n_to_one 2).
 
-Definition loop' limbs weight s c start :=
-  fold_right (loop_body limbs weight s c) start (from_n_to_one (*(limbs - 2 - 1)*)2).
+Definition loop' start :=
+  fold_right loop_body start (from_n_to_one (limbs - 2 - 1)).
 
-Definition mulmod_general limbs weight s c a b :=
+Lemma eval_mod_loop' start :
+  ((Associational.eval (loop' start)) mod (s - c) = (Associational.eval start) mod (s - c))%Z.
+Proof.
+  cbv [loop']. induction (from_n_to_one (limbs - 2 - 1)) as [| i l' IHl'].
+  - reflexivity.
+  - simpl. rewrite eval_mod_loop_body. apply IHl'.
+Qed.
+
+Definition mulmod_general a b :=
   let l := limbs in
   let a_assoc := Positional.to_associational weight limbs a in
   let b_assoc := Positional.to_associational weight limbs b in
@@ -97,21 +198,65 @@ Definition mulmod_general limbs weight s c a b :=
   let r8 := carry' (weight (l - 1)) (Z.div s (weight (l - 1))) r7' in
   let r9 := reduce' s s s c r8 in
   let r10 := carry' (weight 0) (weight 1) r9 in
-  let r11 := loop' l weight s c r10 in
+  let r11 := loop' r10 in
   let r12 := reduce' s (weight (2 * l - 2)) (weight l) c r11 in
   let r13 := carry' (weight (l - 2)) (weight 1) r12 in
   Positional.from_associational weight l r13.
 
 Local Open Scope Z_scope.
 
-Notation "a ** b" := (Zpower_nat a b)
-  (at level 41, right associativity).
+Theorem eval_mod_mulmod_general a b :
+  (Positional.eval weight limbs a * Positional.eval weight limbs b) mod (s - c) =
+  (Positional.eval weight limbs (mulmod_general a b)) mod (s - c).
+Proof.
+  cbv [mulmod_general carry' reduce'].
+  repeat (try rewrite Positional.eval_from_associational;
+          try rewrite Positional.eval_to_associational; 
+          try rewrite Associational.eval_carry; 
+          try rewrite eval_reduce_one;
+          try rewrite eval_carry_down;
+          try rewrite eval_collect_terms;
+          try rewrite eval_mod_loop').
+  rewrite Associational.eval_mul. repeat rewrite Positional.eval_to_associational. reflexivity.
+  all:
+      cbv [weight s base];
+      try apply weight_nz;
+      try apply s_nz;
+      try apply p_nz;
+      try apply weight_0;
+      try apply Z_mod_same_full;
+      try apply limbs_mod_s_0;
+      try apply mod_is_zero;
+      try (remember limbs_gteq_3 as H; lia);
+      try apply base_nz.
+  - apply div_nz.
+    + rewrite Zpower_nat_Z. lia.
+    + rewrite pow_mul. repeat rewrite Zpower_nat_Z. rewrite Nat2Z.inj_mul. rewrite <- Z.pow_le_mono_r_iff.
+      -- remember e_small as H. lia.
+      -- lia.
+      -- lia.
+  - repeat rewrite pow_mul. Search (_ mod (_ / _)). Search ((_ ^ _) / (_ ^ _)). repeat rewrite Zpower_nat_Z.
+    rewrite <- Z.pow_sub_r.
+    + rewrite <- Nat2Z.inj_sub. repeat rewrite <- Zpower_nat_Z. apply mod_is_zero.
+      -- lia.
+      -- lia.
+      -- apply e_small.
+    + lia.
+    + remember e_small as H. lia.
+  - apply div_nz.
+    + repeat rewrite Zpower_nat_Z. lia.
+    + rewrite pow_mul. repeat rewrite Zpower_nat_Z. rewrite Nat2Z.inj_mul. rewrite <- Z.pow_le_mono_r_iff.
+      -- remember e_big as H. lia.
+      -- lia.
+      -- lia.
+Qed.
 
+(*
 Definition s := 2 ** 256.
 
-Definition c := [(2 ** 32 + 977, 1)].
+Definition c := 2 ** 32 + 977.
 
-Definition prime : Z := s - Associational.eval c.
+Definition prime : Z := s - c.
 
 Definition limbs : nat := 5.
 
@@ -128,7 +273,7 @@ Compute (mulmod a b).
 
 Compute (Positional.eval weight limbs (mulmod a b) mod prime).
 Compute (Positional.eval weight limbs (mulmod_general limbs weight s c a b) mod prime).
-Compute ((Positional.eval weight limbs a * Positional.eval weight limbs b) mod prime).
+Compute ((Positional.eval weight limbs a * Positional.eval weight limbs b) mod prime).*)
 
 Local Instance : split_mul_to_opt := None.
 Local Instance : split_multiret_to_opt := None.
@@ -155,13 +300,13 @@ Local Instance : emit_primitives_opt := true.
 Definition input_bounds := Some ((repeat (Some r[0 ~> 2 * m * (2^52 - 1)]%zrange) 4) ++ [Some r[0 ~> 2 * m * (2^48 - 1)]%zrange]).
 Definition output_bounds := Some ((repeat (Some r[0 ~> 2 * M * (2^52 - 1)]%zrange) 4) ++ [Some r[0 ~> 2 * M * (2^48 - 1)]%zrange]).
 
-Definition thing := mulmod_general limbs weight s c.
+Definition thing := mulmod_general.
 
 Time Redirect "log" Compute
   (Pipeline.BoundsPipelineToString
      "fiat_" "bitcoin_mul_u64"
         true true None [64; 128] 64
-        ltac:(let r := Reify (mulmod_general limbs weight s c) in
+        ltac:(let r := Reify (mulmod_general) in
               exact r)
                (fun _ _ => [])
                (input_bounds, (input_bounds, tt))
